src/3d/prelude/extern/EverParse3d.Actions.All.fst
@@ -5,3 +5,5 @@ let _ = EverParse3d.Actions.BackendFlagValue.backend_flag_value
 let ___PUINT8 = unit
 
 let action_field_ptr u = false_elim ()
+
+let action_field_pos_32 u = false_elim ()
