src/3d/InterpreterTarget.fst
@@ -311,6 +311,7 @@ let rec inv_eloc_of_action (a:T.action)
       = match a with
         | Action_return _
         | Action_abort
+        | Action_field_pos_32
         | Action_field_pos_64 -> inv_eloc_nil
         | Action_field_ptr -> Inv_true, Eloc_none, On_success true
         | Action_deref x -> Inv_ptr x, Eloc_none, On_success false
@@ -571,6 +572,9 @@ let rec print_action (mname:string) (a:T.action)
 
         | T.Action_field_pos_64 ->
           "Action_field_pos_64"
+
+        | T.Action_field_pos_32 ->
+          "(Action_field_pos_32 EverParse3d.Actions.BackendFlagValue.backend_flag_value)"
 
         | T.Action_field_ptr ->
           "(Action_field_ptr EverParse3d.Actions.BackendFlagValue.backend_flag_value)"
