src/3d/Target.fsti
@@ -70,6 +70,7 @@ type atomic_action =
   | Action_return of expr
   | Action_abort
   | Action_field_pos_64
+  | Action_field_pos_32
   | Action_field_ptr
   | Action_deref of A.ident
   | Action_assignment : lhs:A.ident -> rhs:expr -> atomic_action
