src/3d/Translate.fst
@@ -599,6 +599,8 @@ let rec translate_action (a:A.action) : ML (T.action & T.decls) =
         T.Action_abort, []
       | Action_field_pos_64 ->
         T.Action_field_pos_64, []
+      | Action_field_pos_32 ->
+        T.Action_field_pos_32, []
       | Action_field_ptr ->
         T.Action_field_ptr, []
       | Action_deref i ->
