src/3d/prelude/EverParse3d.Actions.All.fsti
@@ -15,3 +15,14 @@ val action_field_ptr
       (#[@@@erasable] p:Prelude.parser k t)
       (u:squash (EverParse3d.Actions.BackendFlag.backend_flag == BackendFlagBuffer))
    : action p true_inv eloc_none true ___PUINT8
+
+noextract
+inline_for_extraction
+val action_field_pos_32
+      (#nz:_)
+      (#wk: _)
+      (#k:Prelude.parser_kind nz wk)
+      (#[@@@erasable] t:Type)
+      (#[@@@erasable] p:Prelude.parser k t)
+      (u:squash (EverParse3d.Actions.BackendFlag.backend_flag == BackendFlagBuffer))
+   : action p true_inv eloc_none false FStar.UInt32.t
